Defined a refinement mapping using the network's content.

Isabelle2/R3_Refines_R1.thy
@@ -270,10 +270,113 @@ lemma "is_forward_sim fwd_sim ampr3_ioa ampr1_ioa"
         show ?thesis using 1 2 prems(1,2) apply (auto simp add:sim_defs inv1_def split!:msg.splits packet.splits)
               apply (metis ref_proof_3.axioms(2) ref_proof_3_axioms ref_proof_3_axioms_def)
              apply meson defer
-          apply meson 
-      
-      oops
+          apply meson oops
+end
+
+section {* A fourth attempt *}
   
+locale ref_proof_4 = quorums quorums + amp_r3 leader next_bal as quorums
+  + r1:ampr1_ioa quorums leader
+  for quorums :: "('a::linorder) set set" and leader :: "bal \<Rightarrow> ('a::linorder)" and next_bal as + 
+  fixes ampr3_ioa :: "(('a, 'v) global_state, 'v paxos_action) ioa" 
+    and ampr1_ioa :: "(('v, 'a, 'l) ampr1_state, 'v paxos_action) ioa" 
+  defines "ampr3_ioa \<equiv> ioa" and "ampr1_ioa \<equiv> r1.ioa"
+  fixes a1 a2 a3
+  assumes "a1 \<in> as" and "a2 \<in> as" and "a3 \<in> as" and "a1 \<noteq> a2" and "a3 \<noteq> a2" and "a3 \<noteq> a1"
+begin
+
+interpretation IOA .
+
+lemmas action_defs = propose_def do_2a_def receive_2b_def
+      try_acquire_leadership_def receive_1a_def receive_2a_def receive_1b_def receive_fwd_def
+lemmas init_defs = ampr3_ioa_def ioa_def global_start_def local_start_def
+  ampr1_ioa_def r1.ioa_def r1.start_def r1.start_s_def 
+
+method trans_cases =
+  (simp add:is_trans_def ampr3_ioa_def ioa_def, elim trans_cases)
+
+definition inv1 where inv1_def[inv_proofs_defs]:"inv1 s \<equiv> \<forall> a . acceptors (lstate s a) = as \<and> id (lstate s a) = a"
+lemma inv1:"invariant ampr3_ioa inv1"
+  apply (rule invariantI)
+   apply (simp add:inv1_def init_defs)
+  apply (rm_reachable)
+  apply trans_cases
+         apply (auto simp add:Let_def inv1_def action_defs)
+  done
+declare inv1[invs]
+
+fun extract_vs where 
+  "extract_vs (Fwd v) = {v}"
+| "extract_vs (Phase2a _ _ v) = {v}"
+| "extract_vs (Phase2b _ _ _ v) = {v}"
+| "extract_vs (Phase1b _ _ ff) = {v . \<exists> i b . ff $ i = Some (v,b)}"
+  -- {* Could be @{term "{ff $ i \<bind> (Some o fst) | i . True} \<bind> option_as_set" }*}
+| "extract_vs _ = {}"
+  
+definition propCmd where "propCmd s \<equiv> \<Union> ((\<lambda> p . case p of Packet _ m \<Rightarrow> extract_vs m) ` network s)"
+
+definition propCmd2 where "propCmd2 s \<equiv> {v . \<exists> a \<in> as . 
+  Packet a (Fwd v) \<in> network s 
+  \<or> (\<exists> i b . Packet a (Phase2a i b v) \<in> network s)
+  \<or> (\<exists> a2 \<in> as . \<exists> i b v . Packet a (Phase2b a2 i b v) \<in> network s)
+  \<or> (\<exists> a2 \<in> as . \<exists> b ff i b2 . Packet a (Phase1b a2 b ff) \<in> network s \<and> ff $ i = Some (v,b2))}"
+
+definition ref_map where "ref_map s \<equiv> \<lparr>
+  ampr1_state.propCmd = propCmd s,
+  ballot = \<lambda> a . local_state.ballot (lstate s a),
+  vote = \<lambda> i a b . if (\<exists> a2 v . Packet a2 (Phase2b a i b v) \<in> network s) 
+    then Some (the_elem {v . \<exists> a2 v . Packet a2 (Phase2b a i b v) \<in> network s}) else None,
+  suggestion = \<lambda> i b . if (\<exists> a v. Packet a (Phase2a i b v) \<in> network s) 
+    then Some (the_elem {v . \<exists> a . Packet a (Phase2a i b v) \<in> network s}) else None,
+  onebs = \<lambda> a b . if (\<exists> ff . Packet (leader b) (Phase1b a b ff) \<in> network s) 
+    then Some (the_elem {op$ ff | ff . Packet (leader b) (Phase1b a b ff) \<in> network s}) else None\<rparr>
+
+(* 
+  ampr1_state.propCmd t = propCmd s
+  \<and> ballot t = (\<lambda> a . local_state.ballot (lstate s a))
+  \<and> (\<forall> i b v . suggestion t i b = None \<longleftrightarrow> (\<forall> a . Packet a (Phase2a i b v) \<notin> network s))
+  \<and> (\<forall> i b v . suggestion t i b = Some v \<longleftrightarrow> (\<forall> a . a \<noteq> leader b \<longrightarrow> Packet a (Phase2a i b v) \<in> network s))
+  \<and> (\<forall> i b v a . vote t i a b = None \<longleftrightarrow> (\<forall> a2 . Packet a2 (Phase2b a i b v) \<notin> network s))
+  \<and> (\<forall> i b v a . vote t i a b = Some v \<longleftrightarrow> (\<forall> a2 . a2 \<noteq> a \<longrightarrow> Packet a2 (Phase2b a i b v) \<in> network s))
+  \<and> (\<forall> a b ff . onebs t a b = None \<longleftrightarrow> (Packet (leader b) (Phase1b a b ff) \<notin> network s))
+  \<and> (\<forall> a b f . onebs t a b = Some f \<longleftrightarrow> (Packet (leader b) (Phase1b a b (Abs_finfun f)) \<in> network s))} *)"
+  
+lemmas sim_defs = fwd_sim_def propCmd_def 
+
+lemma "is_forward_sim fwd_sim ampr3_ioa ampr1_ioa"
+  apply (auto simp add:is_forward_sim_def)
+   apply (simp add:init_defs sim_defs)
+   apply (metis ref_proof_3.axioms(2) ref_proof_3_axioms ref_proof_3_axioms_def)
+  apply (insert invs)
+  apply (instantiate_invs)
+  apply (rm_reachable)
+  apply trans_cases
+  subgoal premises prems for s s' t act a v (* Propose *)
+  proof -
+    let ?ef = "[(act, s'\<lparr>ampr1_state.propCmd := insert v (ampr1_state.propCmd s')\<rparr>)]"
+    show ?thesis
+      apply (intro exI[where ?x="?ef"])
+      apply (intro conjI)
+        prefer 3
+        apply (force simp add:trace_match_def trace_def schedule_def externals_def
+          filter_act_def ampr1_ioa_def r1.ioa_def paxos_asig_def Let_def is_trans_def 
+          r1.trans_def split!:if_splits)
+       apply simp
+      subgoal proof (cases "leader (local_state.ballot (lstate s a)) = local_state.id (lstate s a)")
+        case False
+        with prems(1,4) show ?thesis by (simp add:propose_def send_all_def fwd_sim_def propCmd_def)
+      next
+        case True thm prems
+        have 1:"\<And> a . local_state.ballot (lstate t a) = ballot s' a" using prems(1,4) True 
+          by (simp add:do_2a_def propose_def send_all_def fwd_sim_def Let_def propCmd_def)
+        have 2:"network t = network s \<union> {Packet a2 (Phase2a (next_inst (lstate s a)) (local_state.ballot (lstate s a)) v) 
+            | a2 . a2 \<noteq> a \<and> a2 \<in> acceptors (lstate s a)}"
+          using prems(4,2) True
+          by (fastforce simp add:do_2a_def propose_def send_all_def fwd_sim_def propCmd_def Let_def inv1_def)
+        show ?thesis using 1 2 prems(1,2) apply (auto simp add:sim_defs inv1_def split!:msg.splits packet.splits)
+              apply (metis ref_proof_3.axioms(2) ref_proof_3_axioms ref_proof_3_axioms_def)
+             apply meson defer
+          apply meson oops
 end
 
 end
